Changes to typing rules - Datatypes may not bind the same constructor name more than once - Datatype may not bind the same type parameter more than once - Generate a safe (fresh) type variable for the type of matching functions (matchTy) - Require well-kinded result type of constructor signatures - a Let Rec may not bind the same (type) name more than once

src/PlutusIR.v
@@ -903,6 +903,17 @@ Fixpoint splitTy (T : ty) : list ty * ty :=
   | Tr => (nil, Tr)
   end.
 
+Fixpoint returnTy (T : ty) : ty :=
+  match T with
+  | Ty_Fun _ T' => returnTy T'
+  | _           => T
+  end.
+
+Lemma splitTy__returnTy T : snd (splitTy T) = returnTy T.
+Proof.
+  induction T; simpl; intuition.
+Qed.
+
 (* Application spine *)
 Fixpoint spine (t : term) : term * list (term + ty) :=
   match t with
