src/PlutusIR/Semantics/Static/Theorems/Weakening.v
@@ -84,11 +84,12 @@ Module Typing.
     all: try (intros Delta'_0 Gamma'_0 HinclD HinclG).
     all: try (intros Delta'_0 HinclD).
     all: try solve [econstructor; subst; eauto using Kinding.weakening, inclusion_cons, inclusion_append].
-    - (* W_Con *)
+    - (* W_Data *)
       econstructor...
-      subst.
-      intros.
-      eapply H1...
+      + subst.
+        intros.
+        eapply H7...
+      + subst...
   Qed.
 
   Lemma weakening_empty : forall Delta Gamma t T,
